# Flashcards: 7A003--Performance-modeling-and-design-of-computer-systems_processed (Part 40)

**Starting Chapter:** Chapter 25 Transform Analysis. 25.1 Definitions of Transforms and Some Examples

---

#### Definition of Laplace Transform
The Laplace transform, \( \widetilde{X}(s) \), is a method to analyze continuous functions and random variables. It converts a function \( f(t) \) into a new function of the parameter \( s \).

Background context: The Laplace transform is defined as:
\[ L_f(s) = \int_{0}^{\infty} e^{-st} f(t) \, dt \]
For a continuous random variable \( X \), this becomes:
\[ \widetilde{X}(s) = E\left[ e^{-sX} \right] \]

:p What is the definition of the Laplace transform for a continuous function?
??x
The Laplace transform converts a continuous function \( f(t) \) into a new function of parameter \( s \), defined as:
\[ L_f(s) = \int_{0}^{\infty} e^{-st} f(t) \, dt. \]
For a random variable \( X \), the Laplace transform is:
\[ \widetilde{X}(s) = E\left[ e^{-sX} \right]. \]
x??

---

#### Example: Deriving Laplace Transform of Exponential Distribution
Example: Find the Laplace transform of \( X \sim \text{Exp}(\lambda) \).

Background context: The exponential distribution has a probability density function (PDF):
\[ f_X(t) = \lambda e^{-\lambda t}, \quad t \geq 0. \]

:p How do we derive the Laplace transform for an exponentially distributed random variable?
??x
The Laplace transform of \( X \sim \text{Exp}(\lambda) \) is derived as follows:
\[ \widetilde{X}(s) = L_f(s) = \int_{0}^{\infty} e^{-st} \cdot \lambda e^{-\lambda t} \, dt. \]
Simplifying the integral:
\[ \widetilde{X}(s) = \lambda \int_{0}^{\infty} e^{-(s+\lambda)t} \, dt. \]
This is a standard form and can be solved by recognizing it as an exponential integral:
\[ \widetilde{X}(s) = \frac{\lambda}{s + \lambda}. \]

The result shows that the Laplace transform of \( X \sim \text{Exp}(\lambda) \) is \( \frac{\lambda}{s+\lambda} \).
x??

---

#### Definition of z-Transform
The z-transform, \( G_p(z) \), is a method to analyze discrete functions and random variables. It converts a function \( p(i) \) into a new polynomial in the parameter \( z \).

Background context: The z-transform is defined as:
\[ G_p(z) = \sum_{i=0}^{\infty} p(i)z^i. \]
For a discrete random variable \( X \), this becomes:
\[ \hat{X}(z) = E\left[ z^X \right]. \]

:p What is the definition of the z-transform for a discrete function?
??x
The z-transform converts a discrete function \( p(i) \) into a new polynomial in parameter \( z \):
\[ G_p(z) = \sum_{i=0}^{\infty} p(i)z^i. \]
For a random variable \( X \), the z-transform is:
\[ \hat{X}(z) = E\left[ z^X \right]. \]
x??

---

#### Example: Deriving z-Transform of Binomial Distribution
Example: Find the z-transform of \( X \sim \text{Binomial}(n, p) \).

Background context: The binomial distribution has a probability mass function (PMF):
\[ P(X = i) = \binom{n}{i} p^i (1-p)^{n-i}, \quad i = 0, 1, 2, \ldots, n. \]

:p How do we derive the z-transform for a binomially distributed random variable?
??x
The z-transform of \( X \sim \text{Binomial}(n, p) \) is derived as follows:
\[ \hat{X}(z) = G_p(z) = \sum_{i=0}^{n} \binom{n}{i} p^i (1-p)^{n-i} z^i. \]
Recognizing the binomial expansion:
\[ \hat{X}(z) = (pz + (1-p))^n. \]

The result shows that the z-transform of \( X \sim \text{Binomial}(n, p) \) is \( (pz + (1-p))^n \).
x??

---

#### Example: Deriving z-Transform of Geometric Distribution
Example: Find the z-transform of \( X \sim \text{Geometric}(p) \).

Background context: The geometric distribution has a probability mass function (PMF):
\[ P(X = i) = p(1-p)^{i-1}, \quad i = 0, 1, 2, \ldots. \]

:p How do we derive the z-transform for a geometrically distributed random variable?
??x
The z-transform of \( X \sim \text{Geometric}(p) \) is derived as follows:
\[ \hat{X}(z) = G_p(z) = \sum_{i=1}^{\infty} p(1-p)^{i-1} z^i. \]
Recognizing the geometric series sum formula, we can simplify this to:
\[ \hat{X}(z) = \frac{pz}{1 - (1-p)z}. \]

The result shows that the z-transform of \( X \sim \text{Geometric}(p) \) is \( \frac{pz}{1 - (1-p)z} \).
x??

---

#### Example: Deriving z-Transform for Number of Arrivals by Time S
Example: Find the z-transform for the number of arrivals, \( A_S \), by time \( S \), where \( S \) is a random variable and the arrival process is Poisson (λ).

Background context: The Poisson distribution with rate λ has the following properties:
\[ P(A_S = k) = \frac{(\lambda E[S])^k e^{-\lambda E[S]}}{k!}. \]

:p How do we derive the z-transform for the number of arrivals by time S?
??x
The z-transform for \( A_S \), where \( A_S \) is a Poisson process with rate \( \lambda \) and \( S \) is a random variable, can be derived as:
\[ \hat{A_S}(z) = E\left[ z^{A_S} \right] = e^{-\lambda E[S]} \sum_{k=0}^{\infty} \frac{(\lambda E[S])^k}{k!} z^k. \]
Recognizing the exponential series expansion:
\[ \hat{A_S}(z) = e^{-\lambda E[S]} e^{\lambda E[S] z}. \]
Simplifying further:
\[ \hat{A_S}(z) = e^{-\lambda E[S](1-z)}. \]

The result shows that the z-transform for the number of arrivals by time \( S \) is \( e^{-\lambda E[S](1-z)} \).
x??

---

#### Derivation of Z-Transform for AS
Background context: The z-transform is a powerful tool to analyze discrete-time systems. In this example, we derive the z-transform for \( \hat{w}iderAS(z) \), which represents the generating function of the random variable \( AS \). This derivation involves considering the probability mass function (PMF) and using integration.

:p What is the expression for the z-transform of a discrete-time system represented by \( \hat{w}iderAS(z) \)?
??x
The z-transform \( \hat{w}iderAS(z) \) is derived as follows:
\[ \hat{w}iderAS(z) = \sum_{i=0}^{\infty} P\{AS=i\}z^i = \int_0^\infty e^{-\lambda t} (\lambda t)^i i f_S(t) dt z^i \]

This expression uses the PMF of \( AS \), which is given by:
\[ P\{AS=i|S=t\} = \frac{(\lambda t)^i}{i!} e^{-\lambda t} \]
where \( S \) is a continuous random variable with probability density function (PDF) \( f_S(t) \).

By substituting and simplifying, we get:
\[ \hat{w}iderAS(z) = \int_0^\infty e^{-\lambda t} f_S(t) e^{\lambda z t} dt = \int_0^\infty e^{-\lambda (1-z)t} f_S(t) dt \]

This integral is the Laplace transform of \( f_S(t) \) evaluated at \( \lambda(1-z) \), which results in:
\[ \hat{w}iderAS(z) = \tilde{S}(\lambda(1-z)) \]

Here, \( \tilde{S}(s) \) is the Laplace transform of \( f_S(t) \).

??x
The answer with detailed explanations.
This derivation simplifies the complex expression by leveraging the properties of the Laplace transform. The z-transform provides a way to analyze discrete-time systems using continuous-time techniques.

---
#### Getting Moments from Transforms: Peeling the Onion
Background context: In probability theory, moments of a random variable can be derived from its transform (e.g., z-transform or Laplace transform). This method is particularly useful for distributions that are difficult to handle directly. The theorem provides a systematic way to extract moments by taking derivatives.

:p How can we derive the kth moment of a continuous random variable \( X \) using its Laplace transform?
??x
To find the kth moment of a continuous random variable \( X \), we use the derivative of the Laplace transform:
\[ L_f(s) = \int_0^\infty e^{-st} f(t) dt \]

The first few moments can be derived as follows:

- For the 1st moment (mean):
  \[ E[X] = -\frac{d}{ds} L_f(s) \bigg|_{s=0} \]
  
- For the 2nd moment:
  \[ E[X^2] = \frac{d^2}{ds^2} L_f(s) \bigg|_{s=0} \]

This pattern continues, with each higher-order derivative providing a higher moment.

For example, to find the mean of an exponential random variable \( X \sim Exp(\lambda) \):
\[ \hat{X}(s) = L_f(s) = \frac{\lambda}{\lambda + s} \]
Taking the first derivative:
\[ E[X] = -\frac{d}{ds} \left( \frac{\lambda}{\lambda + s} \right) \bigg|_{s=0} = 1/\lambda \]

For the second moment:
\[ E[X^2] = \frac{d^2}{ds^2} \left( \frac{\lambda}{\lambda + s} \right) \bigg|_{s=0} = 2/\lambda^2 \]

Thus, the variance can be calculated as:
\[ Var(X) = E[X^2] - (E[X])^2 = 1/\lambda^2 \]

??x
The answer with detailed explanations.
This method leverages the fact that each derivative of the Laplace transform corresponds to a different moment. By evaluating these derivatives at \( s=0 \), we can extract moments from the transform.

---
#### Derivation of Moments for Discrete Random Variables
Background context: For discrete random variables, the z-transform provides a convenient way to derive moments. The z-transform is defined as:
\[ G(z) = \sum_{i=0}^{\infty} p(i)z^i \]

The derivatives of \( G(z) \) at \( z=1 \) give us the expected values of the products of the random variable.

:p How do we derive the moments for a discrete random variable using its z-transform?
??x
For a discrete random variable \( X \) with probability mass function (PMF) \( p(i) \), the sequence:
\[ G'(z)/v_{|z=1},\, G''(z)/v_{|z=1},\, G'''(z)/v_{|z=1} \]
provides the moments of \( X \).

- The first derivative evaluated at \( z=1 \) gives:
  \[ E[X] = G'(z)/v_{|z=1} \]

- The second derivative evaluated at \( z=1 \) gives:
  \[ E[X(X-1)] = G''(z)/v_{|z=1} \]

- And so on, with higher derivatives providing higher moments.

For example, to find the variance of a geometric random variable \( X \sim Geom(p) \):
\[ \hat{X}(z) = zp/(1-z(1-p)) \]
Taking the second derivative:
\[ E[X(X-1)] = \hat{X}''(z)/v_{|z=1} + E[X] = 2p(1-p)/(1-z(1-p))^3 \bigg|_{z=1} + 1/p \]

Thus, the variance can be calculated as:
\[ Var(X) = E[X^2] - (E[X])^2 = 1 - p / p^2 \]

??x
The answer with detailed explanations.
This method uses the z-transform to systematically derive moments by taking derivatives and evaluating them at \( z=1 \). The geometric random variable example shows how this approach can be applied in practice.

---

#### First Moment of AS Using Transforms
Background context: We are using transforms to compute the first moment (expected value) of \(AS\), where \(S \sim \text{Exp}(\mu)\). The transform technique involves differentiating and applying the chain rule.

:p How do we use transforms to find the expected value of \(AS\)?
??x
To find the expected value of \(AS\), we can use two methods: expanding the transform and then differentiating, or directly differentiating without expanding. Here’s how:

1. **Method 1: Expanding and Differentiating**
   - The transform \(\hat{\widetilde{AS}}(z) = \hat{\widetilde{S}}\left(\lambda (1-z)\right) = \frac{\mu}{\mu + \lambda (1-z)}\).
   - Differentiate with respect to \(z\) and evaluate at \(z=1\):
     \[
     \hat{\widetilde{AS}}'(z) = \frac{d}{dz} \left(\frac{\mu}{\mu + \lambda (1-z)}\right)
     \]
   - Evaluating at \(z=1\):
     \[
     \hat{\widetilde{AS}}'(1) = \frac{\mu \lambda}{(\mu)^2}
     \]

2. **Method 2: Direct Differentiation Without Expanding**
   - The transform is given as:
     \[
     \hat{\widetilde{S}}(z) = \frac{\mu}{\mu + \lambda (1-z)}
     \]
   - Apply the chain rule directly:
     \[
     \hat{\widetilde{AS}}'(z) = \left.\frac{d}{dz} \hat{\widetilde{S}}(\lambda(1-z))\right|_{z=1}
     \]
   - Substitute and differentiate:
     \[
     \left. \frac{d}{dz} \hat{\widetilde{S}}(\lambda (1-z)) \right|_{z=1} = \hat{\widetilde{S}}'(\lambda(1-1)) \cdot (-\lambda) = -E[S] \cdot (-\lambda)
     \]

In both methods, the result is:
\[
E[AS] = \frac{\mu \lambda}{\mu^2} = \frac{\lambda}{\mu}
\]
??x
The expected value of \(AS\) can be calculated using either method, and it results in \(\lambda / \mu\).
```java
// No Java code is necessary for this concept, but if you need to implement the transform logic:
public class TransformExample {
    public double firstMomentOfAS(double mu, double lambda) {
        return lambda / mu;
    }
}
```
x??

---

#### Linearity of Laplace Transforms (Continuous Case)
Background context: We are proving a theorem about the linearity property of Laplace transforms for continuous random variables. Specifically, if \(X\) and \(Y\) are independent with respective p.d.f.s \(x(t)\) and \(y(t)\), then the Laplace transform of their sum is the product of their individual transforms.

:p In proving (25.2), where was independence used?
??x
Independence of \(X\) and \(Y\) was used to separate the expectations in the following step:

\[
\tildewide{Z}(s) = E\left[ e^{-s(X+Y)} \right] = E\left[ e^{-sX} \cdot e^{-sY} \right] = E\left[ e^{-sX} \right] \cdot E\left[ e^{-sY} \right]
\]

This step is only valid if \(X\) and \(Y\) are independent. Without independence, we cannot factor the expectations.
??x
Independence of \(X\) and \(Y\) was used to separate the expectations into a product form, which simplifies the transform calculation.
```java
// No Java code is necessary for this concept, but if you need to implement the logic:
public class LaplaceTransformExample {
    public double laplaceTransformProduct(double muX, double muY) {
        return (muX * muY); // This would be part of a larger transform calculation.
    }
}
```
x??

---

#### Linearity of Z-Transforms (Discrete Case)
Background context: Similar to the Laplace transforms for continuous random variables, we are proving that if \(X\) and \(Y\) are discrete independent random variables, then the z-transform of their sum is the product of their individual z-transforms.

:p How does the proof of (25.3) not require independence?
??x
The proof starts at line (25.6), which involves convolutions rather than direct expectations. The convolution property holds even if \(X\) and \(Y\) are not independent, making the result valid without requiring independence.

In particular:
\[
\tildewide{Z}(z) = \tildewide{X}(z) \cdot \tildewide{Y}(z)
\]
This is derived directly from the convolution of their respective transforms.
??x
The proof does not require \(X\) and \(Y\) to be independent because it relies on the convolution property, which holds for both dependent and independent random variables.

```java
// No Java code is necessary for this concept, but if you need to implement the logic:
public class ZTransformExample {
    public double zTransformProduct(double zTransformX, double zTransformY) {
        return zTransformX * zTransformY;
    }
}
```
x??

