# High-Quality Flashcards: 7A003--Performance-modeling-and-design-of-computer-systems_processed (Part 36)

**Rating threshold:** >= 8/10

**Starting Chapter:** 25.9 Exercises

---

**Rating: 8/10**

#### Z-Transform of Sums of Discrete Random Variables
In this problem, we are dealing with discrete independent random variables \(X\) and \(Y\), and their sum \(Z = X + Y\). The z-transform is a useful tool to analyze such sums.

:p What is the z-transform of \(Z\) if \(X\) and \(Y\) are discrete independent random variables?
??x
The z-transform of \(Z\) can be derived using the property that the z-transform of a sum of independent random variables is the product of their individual z-transforms. Specifically:
\[ \hat{Z}(z) = \hat{X}(z) \cdot \hat{Y}(z) \]

This follows from the definition of the z-transform for discrete random variables, where \( \hat{X}(z) = \sum_{i=0}^{\infty} P(X=i) z^i \).

Here’s a simple example in pseudocode:
```java
// Assuming X and Y are given as arrays representing their probabilities at each value i
double[] probX = ...; // Probabilities for X
double[] probY = ...; // Probabilities for Y

double z = 0.5; // Example value of z
double transformZ = 1.0;

// Calculate the z-transform of Z
for (int i = 0; i < probX.length; i++) {
    for (int j = 0; j < probY.length; j++) {
        transformZ *= probX[i] * probY[j] * Math.pow(z, i + j);
    }
}
```
x??

---

#### Sum of Poissons and Their Distribution
Here we have two independent random variables \(X_1\) and \(X_2\) following a Poisson distribution with parameters \(\lambda_1\) and \(\lambda_2\), respectively. We need to determine the distribution of their sum \(Y = X_1 + X_2\).

:p If \(X_1 \sim \text{Poisson}(\lambda_1)\) and \(X_2 \sim \text{Poisson}(\lambda_2)\), what is the distribution of \(Y\)?
??x
The sum of two independent Poisson random variables is also a Poisson random variable. Specifically, if \(X_1 \sim \text{Poisson}(\lambda_1)\) and \(X_2 \sim \text{Poisson}(\lambda_2)\), then their sum \(Y = X_1 + X_2\) follows a Poisson distribution with parameter \(\lambda_1 + \lambda_2\).

This can be shown using the z-transforms. The z-transform of a Poisson random variable with parameter \(\lambda\) is given by:
\[ \hat{X}(z) = e^{\lambda(z-1)} \]

For \(Y = X_1 + X_2\), we have:
\[ \hat{Y}(z) = \hat{X_1}(z) \cdot \hat{X_2}(z) = e^{\lambda_1(z-1)} \cdot e^{\lambda_2(z-1)} = e^{(\lambda_1 + \lambda_2)(z-1)} \]

This is the z-transform of a Poisson random variable with parameter \(\lambda_1 + \lambda_2\).

x??

---

#### Moments of Poisson Random Variable
We are tasked with deriving \(E[X(X-1)(X-2) \cdots (X-k+1)]\) for \(k = 1, 2, 3, \ldots\) where \(X \sim \text{Poisson}(\lambda)\).

:p What is the expression for \(E[X(X-1)(X-2) \cdots (X-k+1)]\) when \(X \sim \text{Poisson}(\lambda)\)?
??x
For a Poisson random variable \(X\) with parameter \(\lambda\), the factorial moments can be derived using its z-transform. The factorial moment of order \(k\) is given by:
\[ E[X(X-1)(X-2) \cdots (X-k+1)] = k! \cdot \lambda^k \]

This result follows from the properties of the Poisson distribution and its z-transform, which simplifies the calculation of such moments.

x??

---

#### Moments of Binomial Random Variable
In this problem, we need to derive \(E[X(X-1)(X-2) \cdots (X-k+1)]\) for a binomial random variable \(X \sim \text{Binomial}(n, p)\).

:p What is the expression for \(E[X(X-1)(X-1) \cdots (X-k+1)]\) when \(X \sim \text{Binomial}(n, p)\)?
??x
For a binomial random variable \(X \sim \text{Binomial}(n, p)\), the factorial moments can be derived as follows:
\[ E[X(X-1)(X-2) \cdots (X-k+1)] = k! \cdot \binom{n}{k} \cdot p^k \]

This expression is derived using the properties of binomial distributions and their z-transforms, which help in simplifying the calculation of such moments.

x??

---

#### Convergence of Z-Transform
Here we need to prove that if \(|z| \leq 1\), then the z-transform of a discrete non-negative random variable \(X\) converges. The z-transform is defined as:
\[ \hat{X}(z) = \sum_{i=0}^{\infty} p_X(i) z^i \]

:p How do you prove that if \(|z| \leq 1\), then the z-transform of a discrete non-negative random variable \(X\) converges?
??x
To prove the convergence of the z-transform \(\hat{X}(z)\) for \(|z| \leq 1\):

- **Boundedness from Above**: Since \(p_X(i)\) are probabilities, \(0 \leq p_X(i) \leq 1\). Therefore:
\[ |\hat{X}(z)| = \left|\sum_{i=0}^{\infty} p_X(i) z^i \right| \leq \sum_{i=0}^{\infty} |p_X(i) z^i| \leq \sum_{i=0}^{\infty} |z|^i = \frac{1}{1 - |z|} \]
- **Boundedness from Below**: The z-transform cannot be negative, so it is non-negative.

Thus, for \(|z| < 1\), the series converges due to the geometric series test. At \(|z| = 1\), the series may or may not converge depending on the specific values of \(p_X(i)\).

x??

---

#### Transform Analysis in M/M/2 Queue
Here we need to derive the z-transforms and Laplace transforms for an M/M/2 queue with arrival rate \(\lambda\) and service rate \(\mu\).

:p What are the z-transforms and Laplace transform for an M/M/2 queue?
??x
For an M/M/2 queue, the following transforms can be derived:

- **Z-Transform of Number in System**:
\[ \hat{N}(z) = \frac{1 - \rho}{1 - 2\rho + (2-\rho)z} \]
where \(\rho = \lambda / (\mu/2)\).

- **Z-Transform of Queue Length**:
\[ \hat{N_Q}(z) = \frac{\rho^2 z (2 - \rho)}{(1 - 2\rho + (2-\rho)z)(1 - \rho z)} \]

- **Laplace Transform of Queueing Time**:
\[ \tilde{T_Q}(s) = \frac{2\lambda^2 / (\mu(2\mu - \lambda))}{s(s + 2\mu/(\lambda - s))} \]

These transforms are derived from the limiting probabilities and conditional expectations in the M/M/2 queue model.

x??

--- 

Each of these flashcards covers a key concept related to probability distributions, transformations, and queuing theory. They provide both theoretical explanations and practical examples where relevant.

**Rating: 8/10**

#### Deriving πM/G/1 i for M/G/1 Queue

Background context: In the M/G/1 queue, we aim to find the long-run fraction of time that there are \(i\) jobs in the system (\(\pi_{M/G/1}^i\)). For an M/M/1 queue, this was done by creating a continuous-time Markov chain (CTMC). However, for an M/G/1 queue with non-exponential service times, we use an embedded discrete-time Markov chain (DTMC) that considers departures only.

The state of the DTMC is defined as the number of jobs left behind at the time of each departure. Let \(\pi_{\text{embed}}^i\) denote the limiting probability that a departure leaves \(i\) jobs in the system. This is equivalent to the fraction of M/G/1 departures that leave behind \(i\) jobs.

:p How can we derive \(\pi_{M/G/1}^i\) for an M/G/1 queue?
??x
To derive \(\pi_{M/G/1}^i\), we consider the embedded DTMC. The state of this chain is defined as the number of jobs left behind at the time of each departure. We need to find the probabilities \(P_{ij}\) of transitioning from state \(i\) to state \(j\).

For an M/G/1 queue, if \(j < i - 1\), then \(P_{ij} = 0\). For \(j \geq i - 1\), we have:
\[ P_{ij} = P(\text{j arrivals during a job's service time } S) = \int_0^\infty e^{-\lambda x} (\lambda x)^{j-i+1} (j-i+1)! f_S(x) dx. \]

This integral represents the probability of having \(j - i + 1\) arrivals during the service time of a job, which is non-zero only for \(j \geq i - 1\).

:p How do πembed^i and πM/G/1^i compare?
??x
πembed^i and πM/G/1^i are the same. This equivalence holds because the probability that an arrival sees \(i\) jobs is equal to the probability that a departure leaves behind \(i\) jobs, by the Palm–Spitzer formula (PASTA - Poisson Arrivals See Time Averages). Therefore, \(\pi_{embed}^i = \pi_{M/G/1}^i\).

:p What are the steps to derive πembed^i for the M/G/1 queue?
??x
To derive \(\pi_{embed}^i\) for the M/G/1 queue:
1. Consider the embedded DTMC, where states are defined by the number of jobs left behind at each departure.
2. Use the transition probabilities \(P_{ij}\) to set up stationary equations: 
\[ \pi_{embed}^j = \sum_i \pi_{embed}^i P_{ij}. \]
3. Ensure that the sum of all πembed^i equals 1.

:p How do we express πjin terms of aj in the M/G/1 queue?
??x
We can express \(\pi_j\) (where \(j = M/G/1 departure leaves j jobs\)) in terms of \(a_j\), where:
\[ a_j = \int_0^\infty e^{-\lambda x} (\lambda x)^j / j! f_S(x) dx. \]
Thus, for the transition probabilities:
\[ P_{ij} = a_j - i + 1, \quad 1 \leq i \leq j + 1. \]

We have:
\[ \pi_j = \pi_0 a_j + \sum_{i=1}^{j+1} \pi_i a_{j-i+1}. \]
This is the detailed expression for πj in terms of aj.

:p How do we derive z-transform of the number of jobs in system, /hatwideN(z)?
??x
To derive \( \hat{N}(z) = \sum_{i=0}^\infty \pi_{M/G/1}^i z^i \):
1. Express πj in terms of aj: 
\[ \pi_j = \pi_0 a_j + \sum_{i=1}^{j+1} \pi_i a_{j-i+1}. \]
2. Multiply each term by \(z^j\) and sum over all j:
\[ \hat{N}(z) = \sum_{j=0}^\infty \pi_j z^j = \sum_{j=0}^\infty \pi_0 a_j z^j + \sum_{j=0}^\infty \sum_{i=1}^{j+1} \pi_i a_{j-i+1} z^j. \]
3. Recognize the second sum as:
\[ \hat{N}(z) = \frac{\pi_0}{\hat{A}_S(z)} + \sum_{i=1}^\infty \pi_i \sum_{j=i-1}^\infty a_{j-i+1} z^j. \]
4. Simplify the double sum:
\[ \hat{N}(z) = \frac{\pi_0}{\hat{A}_S(z)} + \sum_{i=1}^\infty \pi_i z^{i-1} \sum_{u=0}^\infty a_u z^u. \]
5. Recognize the final sum as:
\[ \hat{N}(z) = \frac{\pi_0}{\hat{A}_S(z)} + \frac{1}{z} (\hat{N}(z) - \pi_0 / \hat{A}_S(z)). \]

Thus, we get:
\[ \hat{N}(z) = \frac{z \pi_0 / \hat{A}_S(z)}{z - \hat{A}_S(z)}. \]

:p How do we determine π0 for the M/G/1 queue?
??x
We know that \( \pi_0 = 1 - \rho \), where \(\rho = \lambda E[S]\) is the fraction of time the server is busy. If you don't know \(\pi_0\), set \(z = 1\) in the expression for \(\hat{N}(z)\):
\[ 1 = \lim_{z \to 1} \frac{\hat{N}(z)}{z - \hat{A}_S(z)}. \]

Using L'Hopital's rule, we find:
\[ 1 = (1 - \rho) \hat{A}_S'(z) / \hat{A}_S(z). \]
Thus,
\[ 1 - \rho = \frac{1}{\hat{A}_S'(1)}. \]

In the case of an M/G/1 queue, this simplifies to:
\[ \pi_0 = 1 - \lambda E[S] = 1 - \rho. \]

---
#### z-transform of Number in System

Background context: After finding πM/G/1 i using the embedded DTMC approach, we derive the z-transform of the number of jobs in the system, \( \hat{N}(z) \).

:p What is the expression for /hatwideN(z)?
??x
The expression for \( \hat{N}(z) \) is:
\[ \hat{N}(z) = \frac{\pi_0}{\hat{A}_S(z)} + \sum_{i=1}^\infty \pi_i z^{i-1} \sum_{u=0}^\infty a_u z^u. \]

Given that \( \pi_0 = 1 - \rho \) and using the properties of the z-transform, we can simplify this to:
\[ \hat{N}(z) = \frac{z \pi_0 / \hat{A}_S(z)}{z - \hat{A}_S(z)}. \]

:p How do we use L'Hopital's rule to find π0?
??x
To find \( \pi_0 \), set \( z = 1 \) in the expression for \( \hat{N}(z) / (z - \hat{A}_S(z)) \):
\[ 1 = \lim_{z \to 1} \frac{\hat{N}(z)}{z - \hat{A}_S(z)}. \]

Using L'Hopital's rule:
\[ 1 = \frac{\pi_0 \hat{A}_S'(1) + (1 - \rho) \hat{A}_S'(1)}{(1 - \hat{A}_S(1))}. \]
Thus,
\[ 1 - \rho = \frac{1}{\hat{A}_S'(1)}. \]

For an M/G/1 queue:
\[ \pi_0 = 1 - \lambda E[S]. \]

---
#### z-transform of A_S(z)

Background context: The z-transform \( \hat{A}_S(z) \) represents the distribution of service times. For an M/G/1 queue, we need to find its value.

:p What is the expression for /hatwideA_S(z)?
??x
The z-transform of the service time distribution \( A_S(z) \) can be expressed as:
\[ \hat{A}_S(z) = \sum_{i=0}^\infty a_i z^i. \]

For an M/G/1 queue, if the service times are generally distributed with mean \( E[S] \), then:
\[ \hat{A}_S(z) = \frac{\phi_A(1 - (1 - z)\lambda)}{z}, \]
where \( \phi_A(s) \) is the Laplace transform of the service time distribution.

:p How do we find /hatwideA_S(z)' at z=1?
??x
To find \( \hat{A}_S'(1) \), differentiate \( \hat{A}_S(z) \):
\[ \hat{A}_S'(z) = \frac{\phi_A'((1 - (1 - z)\lambda))\lambda}{z^2} + \frac{\phi_A(1 - (1 - z)\lambda)}{z}. \]

At \( z = 1 \):
\[ \hat{A}_S'(1) = \phi_A(\lambda). \]

For an exponential service time with rate \( \mu \):
\[ \hat{A}_S(z) = \frac{\mu}{\mu - (1 - z)\lambda}. \]
Thus,
\[ \hat{A}_S'(z) = \frac{\mu^2}{(\mu - (1 - z)\lambda)^2}, \]
and at \( z = 1 \):
\[ \hat{A}_S'(1) = \frac{\mu^2}{\mu^2} = 1. \]

:p How do we use the result to find π0?
??x
Given that:
\[ \pi_0 = 1 - \lambda E[S], \]
and for an M/G/1 queue with exponential service times, \( E[S] = \frac{1}{\mu} \), thus:
\[ \pi_0 = 1 - \rho. \]

:p What is the final expression for /hatwideN(z) in terms of ρ?
??x
The final expression for \( \hat{N}(z) \) in terms of \( \rho \) is:
\[ \hat{N}(z) = \frac{\pi_0 z}{z - (1 - \rho)} = \frac{(1 - \rho)z}{\rho(z - 1 + \rho)}. \]

This expression simplifies to the final form:
\[ \hat{N}(z) = \frac{1 - \rho}{\rho} \cdot \frac{z}{z - (1 - \rho)}. \] 

---
#### Conclusion

The flashcards cover the derivation of \(\pi_{M/G/1}^i\) using an embedded DTMC, the z-transforms for the number of jobs in the system and service time distribution, and how to find \( \pi_0 \) through L'Hopital's rule. The key is understanding the transition probabilities and their implications on the queue behavior.

**Rating: 8/10**

#### Concept: Transform Analysis for N(z)
Background context explaining how we derive \(\hat{N}(z)\) using known formulas and substitutions. The relevant equations are (26.5), (26.6), and (26.7).

:p What is the formula for \(\hat{N}(z)\) derived from?
??x
\[
\hat{N}(z)=\hat{A}_S(z)(1-\rho)\frac{(z-1)}{\hat{A}_S(z)-z}
\]
where \(\hat{A}_S(z)\) is the z-transform of the arrival process within service time \(S\).

x??

#### Concept: Deriving \(\tilde{T}(s)\)
Explanation on how to derive the Laplace transform \(\tilde{T}(s)\) from known results. The key step involves substituting \(T\) for \(S\) in (26.8).

:p What substitution is made to get \(\hat{A}_T(z)\)?
??x
Substitute \(T\) for \(S\) in equation (26.8):
\[
\hat{A}_T(z)=\tilde{T}(\lambda-\lambda z)
\]
This relates the Laplace transform of time in system to the z-transform of arrivals during service.

x??

#### Concept: Deriving \(\tilde{T}(s)\) from \(\hat{N}(z)\)
Explanation on how to derive \(\tilde{T}(s)\) using the relation between \(\hat{A}_T(z)\) and \(\hat{N}(z)\).

:p How is \(\hat{N}(z)\) related to \(\hat{A}_T(z)\)?
??x
\[
\tilde{T}(\lambda-\lambda z)=\hat{A}_T(z)=\hat{N}(z)
\]
By substituting (26.7) into this equation, we get:
\[
\tilde{T}(\lambda-\lambda z)=\frac{\tilde{S}(\lambda-\lambda z)(1-\rho)(1-z)}{\tilde{S}(\lambda-\lambda z)-z}
\]
This allows us to derive \(\tilde{T}(s)\) from \(\hat{N}(z)\).

x??

#### Concept: Change of Variables for \(\tilde{T}(s)\)
Explanation on the change of variables and how it simplifies the expression.

:p What are the steps in changing the variable \(z\) to \(s\)?
??x
Let:
\[
s = \lambda - \lambda z \quad \Rightarrow \quad z = 1 - \frac{s}{\lambda}
\]
Substitute this into (26.11) to get:
\[
\tilde{T}(s)=\frac{\tilde{S}(s)(1-\rho)s/\lambda}{\tilde{S}(s)-1+s/\lambda} = \frac{\tilde{S}(s)(1-\rho)}{\tilde{S}(s)-\lambda + s}
\]
This is the final form of \(\tilde{T}(s)\).

x??

#### Concept: Deriving Laplace Transform of \(T_Q\)
Explanation on how to derive the Laplace transform for the queueing time, \(T_Q\), from \(\tilde{T}(s)\) and \(\tilde{S}(s)\).

:p How do you find \(\tilde{T}_Q(s)\)?
??x
Given:
\[
\tilde{T}(s)=\frac{\tilde{S}(s)(1-\rho)}{\tilde{S}(s)-\lambda + s}
\]
We know \(T = S + T_Q\), thus:
\[
\tilde{T}_Q(s) = \frac{\tilde{T}(s)}{\tilde{S}(s)}
\]
Substituting \(\tilde{T}(s)\):
\[
\tilde{T}_Q(s)=\frac{(1-\rho)s/\lambda}{\tilde{S}(s)-\lambda + s} = \frac{(1-\rho)s/\lambda}{(1-(1-\rho))\tilde{S}(s) - (1-(1-\rho))\lambda + s}
\]
This simplifies to:
\[
\tilde{T}_Q(s)=\frac{s/\lambda}{\tilde{S}(s)-\lambda + s}
\]

x??

#### Concept: Expressing \(\tilde{T}_Q(s)\) in Terms of \(\tilde{\bar{S}}_e(s)\)
Explanation on how to express the Laplace transform of \(T_Q\) using the excess service time's Laplace transform.

:p How do you derive \(\tilde{T}_Q(s)\) from \(\tilde{S}(s)\)?
??x
Recall:
\[
\tilde{\bar{S}}_e(s)=1-\frac{\tilde{S}(s)}{sE[S]}
\]
Using this, we can express:
\[
\tilde{T}_Q(s) = \frac{(1-\rho)s/\lambda}{(1-(1-\rho))\tilde{S}(s) - (1-(1-\rho))\lambda + s} = \frac{s/\lambda}{\tilde{S}(s)-\lambda + s}
\]
Finally:
\[
\tilde{T}_Q(s)=\frac{1-(1-\rho)/\bar{\tilde{S}}_e(s)}{1+1/sE[S]}
\]

x??

---

