# Flashcards: 7A003--Performance-modeling-and-design-of-computer-systems_processed (Part 42)

**Starting Chapter:** Chapter 26 MG1 Transform Analysis. 26.1 The z-Transform of the Number in System

---

#### Deriving πM/G/1 i for M/G/1 Queue

Background context: In the M/G/1 queue, we aim to find the long-run fraction of time that there are \(i\) jobs in the system (\(\pi_{M/G/1}^i\)). For an M/M/1 queue, this was done by creating a continuous-time Markov chain (CTMC). However, for an M/G/1 queue with non-exponential service times, we use an embedded discrete-time Markov chain (DTMC) that considers departures only.

The state of the DTMC is defined as the number of jobs left behind at the time of each departure. Let \(\pi_{\text{embed}}^i\) denote the limiting probability that a departure leaves \(i\) jobs in the system. This is equivalent to the fraction of M/G/1 departures that leave behind \(i\) jobs.

:p How can we derive \(\pi_{M/G/1}^i\) for an M/G/1 queue?
??x
To derive \(\pi_{M/G/1}^i\), we consider the embedded DTMC. The state of this chain is defined as the number of jobs left behind at the time of each departure. We need to find the probabilities \(P_{ij}\) of transitioning from state \(i\) to state \(j\).

For an M/G/1 queue, if \(j < i - 1\), then \(P_{ij} = 0\). For \(j \geq i - 1\), we have:
\[ P_{ij} = P(\text{j arrivals during a job's service time } S) = \int_0^\infty e^{-\lambda x} (\lambda x)^{j-i+1} (j-i+1)! f_S(x) dx. \]

This integral represents the probability of having \(j - i + 1\) arrivals during the service time of a job, which is non-zero only for \(j \geq i - 1\).

:p How do πembed^i and πM/G/1^i compare?
??x
πembed^i and πM/G/1^i are the same. This equivalence holds because the probability that an arrival sees \(i\) jobs is equal to the probability that a departure leaves behind \(i\) jobs, by the Palm–Spitzer formula (PASTA - Poisson Arrivals See Time Averages). Therefore, \(\pi_{embed}^i = \pi_{M/G/1}^i\).

:p What are the steps to derive πembed^i for the M/G/1 queue?
??x
To derive \(\pi_{embed}^i\) for the M/G/1 queue:
1. Consider the embedded DTMC, where states are defined by the number of jobs left behind at each departure.
2. Use the transition probabilities \(P_{ij}\) to set up stationary equations: 
\[ \pi_{embed}^j = \sum_i \pi_{embed}^i P_{ij}. \]
3. Ensure that the sum of all πembed^i equals 1.

:p How do we express πjin terms of aj in the M/G/1 queue?
??x
We can express \(\pi_j\) (where \(j = M/G/1 departure leaves j jobs\)) in terms of \(a_j\), where:
\[ a_j = \int_0^\infty e^{-\lambda x} (\lambda x)^j / j! f_S(x) dx. \]
Thus, for the transition probabilities:
\[ P_{ij} = a_j - i + 1, \quad 1 \leq i \leq j + 1. \]

We have:
\[ \pi_j = \pi_0 a_j + \sum_{i=1}^{j+1} \pi_i a_{j-i+1}. \]
This is the detailed expression for πj in terms of aj.

:p How do we derive z-transform of the number of jobs in system, /hatwideN(z)?
??x
To derive \( \hat{N}(z) = \sum_{i=0}^\infty \pi_{M/G/1}^i z^i \):
1. Express πj in terms of aj: 
\[ \pi_j = \pi_0 a_j + \sum_{i=1}^{j+1} \pi_i a_{j-i+1}. \]
2. Multiply each term by \(z^j\) and sum over all j:
\[ \hat{N}(z) = \sum_{j=0}^\infty \pi_j z^j = \sum_{j=0}^\infty \pi_0 a_j z^j + \sum_{j=0}^\infty \sum_{i=1}^{j+1} \pi_i a_{j-i+1} z^j. \]
3. Recognize the second sum as:
\[ \hat{N}(z) = \frac{\pi_0}{\hat{A}_S(z)} + \sum_{i=1}^\infty \pi_i \sum_{j=i-1}^\infty a_{j-i+1} z^j. \]
4. Simplify the double sum:
\[ \hat{N}(z) = \frac{\pi_0}{\hat{A}_S(z)} + \sum_{i=1}^\infty \pi_i z^{i-1} \sum_{u=0}^\infty a_u z^u. \]
5. Recognize the final sum as:
\[ \hat{N}(z) = \frac{\pi_0}{\hat{A}_S(z)} + \frac{1}{z} (\hat{N}(z) - \pi_0 / \hat{A}_S(z)). \]

Thus, we get:
\[ \hat{N}(z) = \frac{z \pi_0 / \hat{A}_S(z)}{z - \hat{A}_S(z)}. \]

:p How do we determine π0 for the M/G/1 queue?
??x
We know that \( \pi_0 = 1 - \rho \), where \(\rho = \lambda E[S]\) is the fraction of time the server is busy. If you don't know \(\pi_0\), set \(z = 1\) in the expression for \(\hat{N}(z)\):
\[ 1 = \lim_{z \to 1} \frac{\hat{N}(z)}{z - \hat{A}_S(z)}. \]

Using L'Hopital's rule, we find:
\[ 1 = (1 - \rho) \hat{A}_S'(z) / \hat{A}_S(z). \]
Thus,
\[ 1 - \rho = \frac{1}{\hat{A}_S'(1)}. \]

In the case of an M/G/1 queue, this simplifies to:
\[ \pi_0 = 1 - \lambda E[S] = 1 - \rho. \]

---
#### z-transform of Number in System

Background context: After finding πM/G/1 i using the embedded DTMC approach, we derive the z-transform of the number of jobs in the system, \( \hat{N}(z) \).

:p What is the expression for /hatwideN(z)?
??x
The expression for \( \hat{N}(z) \) is:
\[ \hat{N}(z) = \frac{\pi_0}{\hat{A}_S(z)} + \sum_{i=1}^\infty \pi_i z^{i-1} \sum_{u=0}^\infty a_u z^u. \]

Given that \( \pi_0 = 1 - \rho \) and using the properties of the z-transform, we can simplify this to:
\[ \hat{N}(z) = \frac{z \pi_0 / \hat{A}_S(z)}{z - \hat{A}_S(z)}. \]

:p How do we use L'Hopital's rule to find π0?
??x
To find \( \pi_0 \), set \( z = 1 \) in the expression for \( \hat{N}(z) / (z - \hat{A}_S(z)) \):
\[ 1 = \lim_{z \to 1} \frac{\hat{N}(z)}{z - \hat{A}_S(z)}. \]

Using L'Hopital's rule:
\[ 1 = \frac{\pi_0 \hat{A}_S'(1) + (1 - \rho) \hat{A}_S'(1)}{(1 - \hat{A}_S(1))}. \]
Thus,
\[ 1 - \rho = \frac{1}{\hat{A}_S'(1)}. \]

For an M/G/1 queue:
\[ \pi_0 = 1 - \lambda E[S]. \]

---
#### z-transform of A_S(z)

Background context: The z-transform \( \hat{A}_S(z) \) represents the distribution of service times. For an M/G/1 queue, we need to find its value.

:p What is the expression for /hatwideA_S(z)?
??x
The z-transform of the service time distribution \( A_S(z) \) can be expressed as:
\[ \hat{A}_S(z) = \sum_{i=0}^\infty a_i z^i. \]

For an M/G/1 queue, if the service times are generally distributed with mean \( E[S] \), then:
\[ \hat{A}_S(z) = \frac{\phi_A(1 - (1 - z)\lambda)}{z}, \]
where \( \phi_A(s) \) is the Laplace transform of the service time distribution.

:p How do we find /hatwideA_S(z)' at z=1?
??x
To find \( \hat{A}_S'(1) \), differentiate \( \hat{A}_S(z) \):
\[ \hat{A}_S'(z) = \frac{\phi_A'((1 - (1 - z)\lambda))\lambda}{z^2} + \frac{\phi_A(1 - (1 - z)\lambda)}{z}. \]

At \( z = 1 \):
\[ \hat{A}_S'(1) = \phi_A(\lambda). \]

For an exponential service time with rate \( \mu \):
\[ \hat{A}_S(z) = \frac{\mu}{\mu - (1 - z)\lambda}. \]
Thus,
\[ \hat{A}_S'(z) = \frac{\mu^2}{(\mu - (1 - z)\lambda)^2}, \]
and at \( z = 1 \):
\[ \hat{A}_S'(1) = \frac{\mu^2}{\mu^2} = 1. \]

:p How do we use the result to find π0?
??x
Given that:
\[ \pi_0 = 1 - \lambda E[S], \]
and for an M/G/1 queue with exponential service times, \( E[S] = \frac{1}{\mu} \), thus:
\[ \pi_0 = 1 - \rho. \]

:p What is the final expression for /hatwideN(z) in terms of ρ?
??x
The final expression for \( \hat{N}(z) \) in terms of \( \rho \) is:
\[ \hat{N}(z) = \frac{\pi_0 z}{z - (1 - \rho)} = \frac{(1 - \rho)z}{\rho(z - 1 + \rho)}. \]

This expression simplifies to the final form:
\[ \hat{N}(z) = \frac{1 - \rho}{\rho} \cdot \frac{z}{z - (1 - \rho)}. \] 

---
#### Conclusion

The flashcards cover the derivation of \(\pi_{M/G/1}^i\) using an embedded DTMC, the z-transforms for the number of jobs in the system and service time distribution, and how to find \( \pi_0 \) through L'Hopital's rule. The key is understanding the transition probabilities and their implications on the queue behavior.

#### Concept: Transform Analysis for N(z)
Background context explaining how we derive \(\hat{N}(z)\) using known formulas and substitutions. The relevant equations are (26.5), (26.6), and (26.7).

:p What is the formula for \(\hat{N}(z)\) derived from?
??x
\[
\hat{N}(z)=\hat{A}_S(z)(1-\rho)\frac{(z-1)}{\hat{A}_S(z)-z}
\]
where \(\hat{A}_S(z)\) is the z-transform of the arrival process within service time \(S\).

x??

#### Concept: Deriving \(\tilde{T}(s)\)
Explanation on how to derive the Laplace transform \(\tilde{T}(s)\) from known results. The key step involves substituting \(T\) for \(S\) in (26.8).

:p What substitution is made to get \(\hat{A}_T(z)\)?
??x
Substitute \(T\) for \(S\) in equation (26.8):
\[
\hat{A}_T(z)=\tilde{T}(\lambda-\lambda z)
\]
This relates the Laplace transform of time in system to the z-transform of arrivals during service.

x??

#### Concept: Deriving \(\tilde{T}(s)\) from \(\hat{N}(z)\)
Explanation on how to derive \(\tilde{T}(s)\) using the relation between \(\hat{A}_T(z)\) and \(\hat{N}(z)\).

:p How is \(\hat{N}(z)\) related to \(\hat{A}_T(z)\)?
??x
\[
\tilde{T}(\lambda-\lambda z)=\hat{A}_T(z)=\hat{N}(z)
\]
By substituting (26.7) into this equation, we get:
\[
\tilde{T}(\lambda-\lambda z)=\frac{\tilde{S}(\lambda-\lambda z)(1-\rho)(1-z)}{\tilde{S}(\lambda-\lambda z)-z}
\]
This allows us to derive \(\tilde{T}(s)\) from \(\hat{N}(z)\).

x??

#### Concept: Change of Variables for \(\tilde{T}(s)\)
Explanation on the change of variables and how it simplifies the expression.

:p What are the steps in changing the variable \(z\) to \(s\)?
??x
Let:
\[
s = \lambda - \lambda z \quad \Rightarrow \quad z = 1 - \frac{s}{\lambda}
\]
Substitute this into (26.11) to get:
\[
\tilde{T}(s)=\frac{\tilde{S}(s)(1-\rho)s/\lambda}{\tilde{S}(s)-1+s/\lambda} = \frac{\tilde{S}(s)(1-\rho)}{\tilde{S}(s)-\lambda + s}
\]
This is the final form of \(\tilde{T}(s)\).

x??

#### Concept: Deriving Laplace Transform of \(T_Q\)
Explanation on how to derive the Laplace transform for the queueing time, \(T_Q\), from \(\tilde{T}(s)\) and \(\tilde{S}(s)\).

:p How do you find \(\tilde{T}_Q(s)\)?
??x
Given:
\[
\tilde{T}(s)=\frac{\tilde{S}(s)(1-\rho)}{\tilde{S}(s)-\lambda + s}
\]
We know \(T = S + T_Q\), thus:
\[
\tilde{T}_Q(s) = \frac{\tilde{T}(s)}{\tilde{S}(s)}
\]
Substituting \(\tilde{T}(s)\):
\[
\tilde{T}_Q(s)=\frac{(1-\rho)s/\lambda}{\tilde{S}(s)-\lambda + s} = \frac{(1-\rho)s/\lambda}{(1-(1-\rho))\tilde{S}(s) - (1-(1-\rho))\lambda + s}
\]
This simplifies to:
\[
\tilde{T}_Q(s)=\frac{s/\lambda}{\tilde{S}(s)-\lambda + s}
\]

x??

#### Concept: Expressing \(\tilde{T}_Q(s)\) in Terms of \(\tilde{\bar{S}}_e(s)\)
Explanation on how to express the Laplace transform of \(T_Q\) using the excess service time's Laplace transform.

:p How do you derive \(\tilde{T}_Q(s)\) from \(\tilde{S}(s)\)?
??x
Recall:
\[
\tilde{\bar{S}}_e(s)=1-\frac{\tilde{S}(s)}{sE[S]}
\]
Using this, we can express:
\[
\tilde{T}_Q(s) = \frac{(1-\rho)s/\lambda}{(1-(1-\rho))\tilde{S}(s) - (1-(1-\rho))\lambda + s} = \frac{s/\lambda}{\tilde{S}(s)-\lambda + s}
\]
Finally:
\[
\tilde{T}_Q(s)=\frac{1-(1-\rho)/\bar{\tilde{S}}_e(s)}{1+1/sE[S]}
\]

x??

---

#### M/G/1 Queue: Job Size Distribution
Background context explaining the concept of an M/G/1 queue and its job size distribution. The job sizes \(S\) follow a two-phase exponential distribution:
\[ S \sim \begin{cases} 
\text{Exp}(\mu_1) & \text{with probability } p \\
\text{Exp}(\mu_2) & \text{with probability } 1-p 
\end{cases} \]
This means that the job size can be either exponentially distributed with rate \(\mu_1\) or \(\mu_2\), depending on a probability \(p\).

:p What is the distribution of job sizes in an M/G/1 queue?
??x
The job sizes \(S\) follow a mixture of two exponential distributions, each with its own rate parameter. Specifically:
- With probability \(p\), the job size follows \(\text{Exp}(\mu_1)\).
- With probability \(1-p\), the job size follows \(\text{Exp}(\mu_2)\).

This can be represented as a weighted sum of two exponential distributions.
x??

#### Deriving \(E[TQ]\) for M/G/1
Background context explaining how to derive the expected time in queue (\(E[TQ]\)) for an M/G/1 queue, given that job sizes follow an H2 distribution.

:p Derive \(E[TQ]\) for the M/G/1 queue.
??x
To derive \(E[TQ]\), we need to consider the properties of the system and the job size distribution. The expected time in queue can be found by analyzing the steady-state behavior of the system, taking into account the different rates \(\mu_1\) and \(\mu_2\).

The formula for \(E[TQ]\) involves solving a balance equation or using known results from queueing theory. For an M/G/1 queue with job sizes following an H2 distribution:
\[ E[TQ] = \frac{1}{\lambda} + p \cdot \frac{1}{\mu_1 - \lambda} + (1-p) \cdot \frac{1}{\mu_2 - \lambda} \]
where \(\lambda\) is the arrival rate.

Here's a simplified approach to derive \(E[TQ]\):
```java
public class MGA1Queue {
    private double mu1, mu2, p;
    
    public MGA1Queue(double mu1, double mu2, double p) {
        this.mu1 = mu1;
        this.mu2 = mu2;
        this.p = p;
    }
    
    public double expectedTimeInQueue(double lambda) {
        return 1.0 / lambda + p * (1.0 / (mu1 - lambda)) + (1 - p) * (1.0 / (mu2 - lambda));
    }
}
```
x??

#### Deriving \(\tilde{TQ}(s)\) for M/G/1
Background context explaining the Laplace transform of the time in queue (\(\tilde{TQ}(s)\)) for an M/G/1 queue, given that job sizes follow an H2 distribution.

:p Derive \(\tilde{TQ}(s)\) for the M/G/1 queue.
??x
To derive \(\tilde{TQ}(s)\), we need to use the Laplace transform properties and the known results from queueing theory. For an M/G/1 queue, the Laplace transform of the time in queue can be derived as:
\[ \tilde{TQ}(s) = \frac{c_0 + c_1 s}{\lambda (s - 1)} \]
where \(c_0\) and \(c_1\) are constants that depend on the parameters of the system, including \(\mu_1\), \(\mu_2\), and \(p\).

Here's a pseudocode approach to derive \(\tilde{TQ}(s)\):
```java
public class MG1Queue {
    private double mu1, mu2, p;
    
    public MG1Queue(double mu1, double mu2, double p) {
        this.mu1 = mu1;
        this.mu2 = mu2;
        this.p = p;
    }
    
    public double laplaceTransformInQueue(double s, double lambda) {
        // Constants based on the system parameters
        double c0 = ...;  // Calculate based on \mu_1, \mu_2, and p
        double c1 = ...;  // Calculate based on \mu_1, \mu_2, and p
        
        return (c0 + c1 * s) / (lambda * (s - 1));
    }
}
```
x??

#### Variance of Response Time for M/G/1
Background context explaining how to derive the variance of response time (\(\text{Var}(TQ)\)) using the Laplace transform \(\tilde{TQ}(s)\) for an M/G/1 queue.

:p Derive \(\text{Var}(TQ)\) for the M/G/1 queue.
??x
To derive the variance of the response time, we need to differentiate \(\tilde{TQ}(s)\) and use known results from Laplace transforms. The variance can be derived as:
\[ \text{Var}(TQ) = -\left[ \frac{\partial^2}{\partial s^2} \tilde{TQ}(s) \right]_{s=0} + E[TQ]^2 \]

Here's a pseudocode approach to derive the variance:
```java
public class MG1Queue {
    // ... previous methods ...
    
    public double varianceOfResponseTime(double lambda, double s) {
        double c0 = ...;  // Calculate based on \mu_1, \mu_2, and p
        double c1 = ...;  // Calculate based on \mu_1, \mu_2, and p
        
        // Laplace transform of TQ
        double tTQs = (c0 + c1 * s) / (lambda * (s - 1));
        
        // Differentiate twice with respect to s
        double secondDerivative = ...;  // Calculate the second derivative at s=0
        
        return -secondDerivative + Math.pow(expectedTimeInQueue(lambda), 2);
    }
}
```
x??

#### z-Transform of Number of Jobs Queued
Background context explaining how to derive the z-transform of the number of jobs queued (\(\hat{\tilde{N}}_Q(z)\)) from the z-transform of the total number of jobs in the system (\(\hat{N}(z)\)).

:p Derive \(\hat{\tilde{N}}_Q(z)\) from \(\hat{N}(z)\).
??x
To derive the z-transform of the number of jobs queued, we need to subtract the z-transform of the number of jobs in service from the total z-transform. If \(\hat{N}(z)\) is the z-transform of the total number of jobs in the system, then:
\[ \hat{\tilde{N}}_Q(z) = \hat{N}(z) - z^{-1} G'(0) \]
where \(G'(0)\) is the first derivative of the generating function at 0.

Here's a pseudocode approach to derive \(\hat{\tilde{N}}_Q(z)\):
```java
public class MG1Queue {
    // ... previous methods ...
    
    public double zTransformNumberOfJobsQueued(double z, double lambda) {
        double totalJobs = ...;  // Calculate based on the system parameters
        double derivativeAtZero = ...;  // Calculate G'(0)
        
        return totalJobs - (z - 1);
    }
}
```
x??

#### Distributional Little's Law for M/G/1 and M/G/c
Background context explaining the distributional version of Little's law and its application to M/G/1 and M/G/c queues.

:p Derive Distributional Little's Law for M/G/1 and M/G/c.
??x
Distributional Little's Law states that:
\[ E[N(N-1)(N-2)\cdots(N-k+1)] = \lambda^k E[T_k] \]
for all integers \( k \geq 1 \). This law relates the moments of the number of jobs in the system to the moments of the response time.

For an M/G/1 queue:
\[ E[N(N-1)(N-2)\cdots(N-k+1)] = \lambda^k E[T_k] \]
where \( T_k \) is the k-th moment of the response time.

Here's a pseudocode approach to derive the moments using Distributional Little's Law:
```java
public class MG1Queue {
    // ... previous methods ...
    
    public double distributionalLittleLawMoment(double lambda, int k) {
        return Math.pow(lambda, k) * expectedResponseTimeMoment(k);
    }
}
```
x??

#### M/M/2 Transform
Background context explaining the transformation from \(\hat{N}(z)\) to \(\tilde{TQ}(s)\) for an M/G/1 queue and applying this technique to the M/M/2 queue.

:p Derive \(\hat{\tilde{N}}_Q(z)\) for the M/M/2 queue.
??x
To derive \(\hat{\tilde{N}}_Q(z)\) for the M/M/2 queue, we follow a similar approach as used for the M/G/1 queue. First, we need to find \(\hat{\tilde{N}}_Q(z)\), then convert it to the waiting time transform \(\tilde{TQ}(s)\).

The steps involve:
1. Deriving \(\hat{\tilde{N}}_Q(z)\) using known results or matrix-analytic methods.
2. Converting \(\hat{\tilde{N}}_Q(z)\) to \(\tilde{TQ}(s)\).

Here's a pseudocode approach to derive \(\hat{\tilde{N}}_Q(z)\):
```java
public class MM2Queue {
    // ... previous methods ...
    
    public double zTransformNumberOfJobsQueued(double z, double lambda) {
        // Use matrix-analytic methods or known results
        return ...;
    }
}
```
x??

---
These flashcards cover key concepts and provide context and explanations to aid in understanding the material.

