# Flashcards: 7A003--Performance-modeling-and-design-of-computer-systems_processed (Part 40)

**Starting Chapter:** Chapter 25 Transform Analysis. 25.1 Definitions of Transforms and Some Examples

---

#### Laplace Transform Definition and Examples
Background context explaining the concept. The Laplace transform, \( \tilde{X}(s) \), of a continuous random variable (r.v.) \( X \) is defined as:
\[ \tilde{X}(s) = Lf(s) = \int_0^\infty e^{-st} f_X(t) dt \]
where \( f_X(t) \) is the probability density function (p.d.f.) of \( X \). When speaking of the Laplace transform of a continuous r.v., we refer to it as \( \tilde{X}(s) = Lf(s) = E[e^{-sX}] \).

:p What is the definition of the Laplace transform for a continuous random variable?
??x
The Laplace transform, \( \tilde{X}(s) \), of a continuous random variable \( X \) with p.d.f. \( f_X(t) \) is defined as:
\[ \tilde{X}(s) = Lf(s) = \int_0^\infty e^{-st} f_X(t) dt \]
This can also be written as the expected value of \( e^{-sX} \):
\[ E[e^{-sX}] \]
x??

---
#### Laplace Transform Example: Exponential Distribution
Background context explaining the concept. An example is provided to illustrate how to derive the Laplace transform for an exponential distribution with rate parameter \( \lambda \).

:p Derive the Laplace transform of a random variable \( X \sim Exp(\lambda) \).
??x
The Laplace transform of \( X \sim Exp(\lambda) \) can be derived as follows:
\[ \tilde{X}(s) = Lf(s) = \int_0^\infty e^{-st} \lambda e^{-\lambda t} dt = \frac{\lambda}{s + \lambda} \]
The integral simplifies to the result above because \( e^{-(s+\lambda)t} \) integrates to \( \frac{1}{s + \lambda} \).

:p Derive the Laplace transform of a constant random variable.
??x
The Laplace transform of a constant random variable \( X = a \) is:
\[ \tilde{X}(s) = e^{-sa} \]
This result comes from integrating \( 1 \cdot f(t) \) where \( f(t) = 0 \) for all \( t \neq a \).

:p Derive the Laplace transform of a uniformly distributed random variable.
??x
The Laplace transform of \( X \sim Uniform(a, b) \) is:
\[ \tilde{X}(s) = \int_0^\infty e^{-st} f_X(t) dt = \frac{-e^{-sb} - e^{-sa}}{s(b-a)} \]
This can be simplified to:
\[ \frac{e^{-sa} - e^{-sb}}{s(b-a)} \]

:p Why does the Laplace transform converge?
??x
The Laplace transform converges if \( f(t) \) is a p.d.f. of some non-negative random variable and \( s \geq 0 \). To see why, note that:
\[ e^{-t} \leq 1 \text{ for all } t \geq 0 \]
Thus,
\[ e^{-st} \leq 1 \text{ if } s \geq 0 \]
This implies:
\[ Lf(s) = \int_0^\infty e^{-st} f(t) dt \leq \int_0^\infty 1 \cdot f(t) dt = 1 \]
Hence, the Laplace transform converges.

x??

---
#### Z-Transform Definition and Examples
Background context explaining the concept. The z-transform \( Gp(z) \) of a discrete function \( p(i) \) is defined as:
\[ Gp(z) = \sum_{i=0}^\infty p(i) z^i \]
When referring to a discrete random variable (r.v.) \( X \), we are dealing with the z-transform of its probability mass function (p.m.f.). We write \( \hat{X}(z) \) to denote this transform. For a discrete r.v., if \( p(i) \) is the p.m.f., then:
\[ \hat{X}(z) = Gp(z) = E[z^X] \]

:p What is the definition of the z-transform for a discrete random variable?
??x
The z-transform, \( \hat{X}(z) \), of a discrete r.v. \( X \) with p.m.f. \( p_X(i) \) is defined as:
\[ \hat{X}(z) = Gp(z) = \sum_{i=0}^\infty p_X(i) z^i \]
This can also be written in terms of the expected value as:
\[ E[z^X] \]

:p Derive the z-transform of a binomial distribution.
??x
The z-transform of \( X \sim Binomial(n, p) \) is derived as follows:
\[ \hat{X}(z) = Gp(z) = \sum_{i=0}^n \binom{n}{i} p^i (1-p)^{n-i} z^i \]
This can be simplified to:
\[ (zp + 1 - p)^n \]

:p Derive the z-transform of a geometric distribution.
??x
The z-transform of \( X \sim Geometric(p) \) is derived as follows:
\[ \hat{X}(z) = Gp(z) = \sum_{i=1}^\infty p (1-p)^{i-1} z^i = p z \sum_{i=0}^\infty (z(1-p))^i = \frac{pz}{1 - z(1-p)} \]

:p Derive the z-transform of a Poisson process with parameter \( \lambda t \) for the number of arrivals by time \( t \).
??x
The z-transform of \( A_t \), the number of arrivals by time \( t \) in a Poisson process with rate \( \lambda \), is:
\[ \hat{A_t}(z) = e^{-\lambda t} \sum_{i=0}^\infty (\lambda t z)^i i! = e^{-\lambda t} (1 - z)^{-1} = e^{-\lambda t} (1 - z)^{-1} \]

:p Derive the z-transform of a Poisson process with parameter \( \lambda S \) for the number of arrivals by time \( S \), where \( S \) is a random variable.
??x
The z-transform of \( A_S \), the number of arrivals by time \( S \) in a Poisson process with rate \( \lambda \), is:
\[ \hat{A_S}(z) = e^{-\lambda E[S]} (1 - z)^{-1} \]
where \( E[S] \) is the expected value of the random variable \( S \).

x??

---

#### Z-Transform of a Discrete Random Variable AS
Background context: The z-transform provides a way to analyze discrete random variables. It is defined as:
\[
\hat{A_S}(z) = \sum_{i=0}^{\infty} P(A_S=i)z^i
\]
Where \(P(A_S=i)\) is the probability that the discrete random variable \(A_S\) takes on the value \(i\).

Given the provided equation, we can derive \(\hat{A_S}(z)\) by substituting the conditional probabilities and integrating over time:
\[
\hat{A_S}(z) = \sum_{i=0}^{\infty} P(A_S=i|S=t)f_S(t)dt \cdot z^i
\]
Where \(f_S(t)\) is the probability density function (pdf) of \(S\).

The provided solution simplifies this to:
\[
\hat{A_S}(z) = \int_{0}^{\infty} e^{-\lambda t}(\lambda t)^i \frac{i}{f_S(t)} dt \cdot z^i
\]
This can be further simplified and integrated over time, leading to the final expression:
\[
\hat{A_S}(z) = \tilde{S}(\lambda(1-z))
\]

:p What is the z-transform of a discrete random variable \(A_S\)?
??x
The z-transform of a discrete random variable \(A_S\) can be derived by summing up the weighted probabilities, where each probability is multiplied by the corresponding power of \(z\). The detailed derivation involves integrating over time with respect to the conditional probability and simplifying using exponential functions.
```java
// Pseudocode for deriving z-transform
public class ZTransform {
    public double getZTransform(double lambda, double z, Function<Double, Double> fS) {
        // Integrate e^(-lambda*t) * (lambda*t)^i * i / fS(t) * z^i over t from 0 to infinity
        return integrate(lambda, z, fS);
    }

    private double integrate(double lambda, double z, Function<Double, Double> fS) {
        // Placeholder for integration logic
        return 1; // Dummy value for illustration
    }
}
```
x??

---

#### Moments from Transforms: Peeling the Onion Theorem
Background context: This theorem provides a method to compute the moments of a continuous random variable \(X\) using its Laplace transform. Specifically, it states that:
\[
E[X^n] = (-1)^n \frac{d^n L_f(s)}{ds^n} \bigg|_{s=0}
\]
Where \(L_f(s)\) is the Laplace transform of the pdf \(f(t)\).

The proof involves expanding \(e^{-st}\) and applying it to the integral form of the Laplace transform, then taking derivatives to extract moments.

:p How can we use the Laplace transform to find the moments of a continuous random variable?
??x
We can use the Laplace transform to find the moments of a continuous random variable by differentiating the transform with respect to \(s\) and evaluating at \(s=0\). For example, the first moment (mean) is obtained by taking the negative derivative once, the second moment involves twice differentiation, and so on.

```java
// Pseudocode for computing moments using Laplace transform
public class MomentCalculator {
    public double computeMoments(double lambda, Function<Double, Double> fS) {
        // Compute L_f(s)
        double Lf = integrate(0, Math.pow(lambda, -1), fS);
        
        // Differentiate and evaluate at s=0 to get the moments
        return differentiate(Lf, 0); // Placeholder for differentiation logic
    }

    private double differentiate(double value, double point) {
        // Placeholder for differentiation logic
        return 0; // Dummy value for illustration
    }
}
```
x??

---

#### Moments from Transforms: Discrete Random Variable
Background context: For a discrete random variable \(X\) with probability mass function (pmf) \(p(i)\), the moments can be derived from the generating function \(\hat{G}(z)\). Specifically:
\[
\hat{G}'(z) \bigg|_{z=1} = E[X]
\]
\[
\hat{G}''(z) \bigg|_{z=1} = E[X(X-1)]
\]
\[
\hat{G}'''(z) \bigg|_{z=1} = E[X(X-1)(X-2)]
\]
And generally:
\[
\hat{G}^{(n)}(z) \bigg|_{z=1} = E[X(X-1)(X-2)\cdots (X-n+1)]
\]

The proof involves differentiating the generating function and evaluating at \(z=1\).

:p How can we compute the moments of a discrete random variable using its transform?
??x
We can compute the moments of a discrete random variable by differentiating its generating function \(\hat{G}(z)\) and evaluating it at \(z=1\). For example, to find the first moment (mean), we differentiate once; for the second moment, twice; and so on.

```java
// Pseudocode for computing moments using transform
public class DiscreteMomentCalculator {
    public double computeMoments(Function<Double, Double> p) {
        // Compute G(z)
        double G = sum(p);
        
        // Differentiate and evaluate at z=1 to get the moments
        return differentiate(G, 0); // Placeholder for differentiation logic
    }

    private double differentiate(double value, double point) {
        // Placeholder for differentiation logic
        return 0; // Dummy value for illustration
    }
}
```
x??

---

#### Example: Exponential Distribution (Exp(Î»))
Background context: The example provided shows how to compute the moments of an exponential random variable \(X \sim Exp(\lambda)\) using its Laplace transform. The Laplace transform is given by:
\[
\hat{X}(s) = \frac{\lambda}{\lambda + s}
\]
The mean and higher-order moments are derived by taking derivatives and evaluating at \(s=0\).

:p How can we derive the kth moment of an exponential random variable?
??x
To derive the kth moment of an exponential random variable \(X \sim Exp(\lambda)\), we use its Laplace transform:
\[
\hat{X}(s) = \frac{\lambda}{\lambda + s}
\]
By taking derivatives and evaluating at \(s=0\), we can find each moment. For example, the first moment (mean):
\[
E[X] = -\frac{d\hat{X}(s)}{ds} \bigg|_{s=0} = \lambda
\]
The second moment:
\[
E[X^2] = \frac{d^2\hat{X}(s)}{ds^2} \bigg|_{s=0} = 2\lambda^2
\]
And the kth moment:
\[
E[X^k] = (-1)^k \frac{d^k\hat{X}(s)}{ds^k} \bigg|_{s=0} = k \lambda^{k-1}
\]

```java
// Pseudocode for computing moments of exponential distribution
public class ExponentialMoments {
    public double computeMoments(double lambda, int k) {
        // Derivative logic here
        return k * Math.pow(lambda, k - 1); // Placeholder for actual derivative calculation
    }
}
```
x??

---

#### Example: Geometric Distribution (Geo(p))
Background context: The example provided demonstrates how to compute the variance of a geometric random variable \(X \sim Geo(p)\) using its z-transform. The z-transform is given by:
\[
\hat{X}(z) = \frac{p z}{1 - z(1-p)}
\]
By taking derivatives and evaluating at \(z=1\), we can find the mean and variance.

:p How can we derive the variance of a geometric random variable?
??x
To derive the variance of a geometric random variable \(X \sim Geo(p)\), we use its z-transform:
\[
\hat{X}(z) = \frac{p z}{1 - z(1-p)}
\]
First, compute the first moment (mean):
\[
E[X] = \frac{d\hat{X}(z)}{dz} \bigg|_{z=1} = 1/p
\]
Then, compute the second moment:
\[
E[X^2] = \hat{X}''(z) \bigg|_{z=1} + E[X] = (2 - p)/(p^2)
\]
Finally, the variance is:
\[
Var(X) = E[X^2] - (E[X])^2 = 1/p^2 - 1/p^2 = 1 - p / p^2
\]

```java
// Pseudocode for computing variance of geometric distribution
public class GeometricVariance {
    public double computeVariance(double p) {
        // Compute E[X] and E[X^2]
        double mean = 1 / p;
        double secondMoment = (2 - p) / Math.pow(p, 2);
        
        // Variance calculation
        return secondMoment - Math.pow(mean, 2); // Placeholder for actual computation
    }
}
```
x??

#### First Moment of AS Using Transforms

Background context: This concept involves using transforms to compute the first moment (expected value) of \(AS\), where \(S \sim \text{Exp}(\mu)\). The expected value is derived by differentiating the transform and evaluating it at a specific point.

:p How do we use transforms to compute the first moment \(E[AS]\)?
??x
We can use two methods: expanding the transform and then differentiating, or directly applying differentiation without expanding. Both methods yield the same result, \(\frac{\lambda}{\mu}\).

1. **Method 1: Expanding and Differentiating**
   - Start with the Laplace transform of \(S\): \(\hat{W}_{\tilde{S}}(z) = \frac{\mu}{\mu + \lambda(1-z)}\).
   - Differentiate this to get \(\frac{d}{dz} \hat{W}_{\tilde{S}}(z)\).
   - Evaluate at \(z=1\) to find the first moment.

2. **Method 2: Direct Differentiation**
   - Use the chain rule directly on \(\hat{W}_{\tilde{S}}(\lambda(1-z))\).
   - Derive and evaluate as shown in the text.
??x
The expected value is computed by differentiating the transform of \(S\) with respect to \(z\), evaluating at \(z=1\). Both methods confirm that \(E[AS] = \frac{\lambda}{\mu}\).

```java
// Pseudocode for Method 2
public class MomentCalculation {
    public double computeExpectedValue(double lambda, double mu) {
        return lambda / mu;
    }
}
```
x??

---

#### Linearity of Transforms (Theorem 25.7)

Background context: This theorem states that if \(X\) and \(Y\) are independent continuous random variables with probability density functions \(f_X(t)\) and \(f_Y(t)\), then the Laplace transform of their sum \(Z = X + Y\) is given by \(\hat{W}_{\tilde{Z}}(s) = \hat{W}_{\tilde{X}}(s) \cdot \hat{W}_{\tilde{Y}}(s)\).

:p How does the linearity of transforms apply to the sum of two independent random variables?
??x
The linearity of transforms means that if \(X\) and \(Y\) are independent, then the Laplace transform of their sum \(Z = X + Y\) is simply the product of their individual Laplace transforms.

If \(X_1, \ldots, X_n\) are i.i.d. random variables with common Laplace transform \(\hat{W}_{\tilde{X}}(s)\), then for \(Z = X_1 + \cdots + X_n\):

\[ \hat{W}_{\tilde{Z}}(s) = (\hat{W}_{\tilde{X}}(s))^n. \]

This is derived from the convolution of their individual transforms.
??x
The Laplace transform of the sum of independent random variables equals the product of their individual transforms.

```java
// Pseudocode for Summing Independent Variables
public class TransformSum {
    public double computeLaplaceTransform(int n, double s) {
        return Math.pow(laplaceTransformOfX(s), n);
    }
    
    private double laplaceTransformOfX(double s) {
        // Return the Laplace transform of X at s
    }
}
```
x??

---

#### Proof of Linearity (Equation 25.2)

Background context: This proof involves showing that for independent random variables \(X\) and \(Y\), the Laplace transform of their sum is the product of their individual transforms.

:p Where was the independence condition used in proving Theorem 25.7?
??x
The independence of \(X\) and \(Y\) was crucial when moving from equation (25.5) to equation (25.6). Specifically, it allowed us to factor out \(y(k)\) from the inner integral.

Without independence, this step would not be valid.
??x
Independence was necessary because only then can we separate the integrals and simplify as shown in the proof.

```java
// Pseudocode for Independence Check
public class IndependenceCheck {
    public boolean areIndependent(RandomVariable X, RandomVariable Y) {
        // Logic to check if X and Y are independent
        return true; // Placeholder logic
    }
}
```
x??

---

#### Convolution and Laplace Transforms (Equation 25.3)

Background context: This theorem extends the concept of transform linearity to non-independent random variables, using convolution.

:p How does the proof of Equation 25.3 handle non-independent random variables?
??x
The proof starts from equation (25.6), where it directly manipulates the Laplace transform without needing independence between \(X\) and \(Y\).

For any random variables \(X\) and \(Y\), if we define their convolution as \(g(t) = \int_0^t x(t-k)y(k)dk\), then:

\[ L_g(s) = L_{x \otimes y}(s) = L_x(s)L_y(s). \]

This is valid even when the variables are not independent, although in practice \(g(t)\) only equals \(z(t)\) if \(X\) and \(Y\) are independent.
??x
The proof of Equation 25.3 does not require independence because it starts from equation (25.6), which directly manipulates the transform without separation.

```java
// Pseudocode for Convolution Proof
public class ConvolutionProof {
    public double computeLaplaceTransform(double s, Function x, Function y) {
        // Logic to compute the Laplace transform using convolution
        return laplaceTransformOfX(s) * laplaceTransformOfY(s);
    }
    
    private double laplaceTransformOfX(double s) {
        // Return the Laplace transform of X at s
    }
    
    private double laplaceTransformOfY(double s) {
        // Return the Laplace transform of Y at s
    }
}
```
x??

---

#### Z-Transform for Discrete Variables

Background context: The z-transform is a similar concept to the Laplace transform but used for discrete random variables. For independent discrete random variables \(X\) and \(Y\), if \(Z = X + Y\), then:

\[ \hat{W}_{\tilde{Z}}(z) = \hat{W}_{\tilde{X}}(z) \cdot \hat{W}_{\tilde{Y}}(z). \]

:p How is the z-transform applied to the sum of discrete independent random variables?
??x
The z-transform of the sum \(Z\) of two independent discrete random variables \(X\) and \(Y\) is simply the product of their individual z-transforms.

If \(X_1, \ldots, X_n\) are i.i.d. with common z-transform \(\hat{W}_{\tilde{X}}(z)\), then for \(Z = X_1 + \cdots + X_n\):

\[ \hat{W}_{\tilde{Z}}(z) = (\hat{W}_{\tilde{X}}(z))^n. \]

This is derived from the convolution of their individual transforms in the discrete domain.
??x
The z-transform of the sum of independent discrete random variables equals the product of their individual z-transforms.

```java
// Pseudocode for Z-Transform Sum
public class ZTransformSum {
    public double computeZTransform(int n, double z) {
        return Math.pow(zTransformOfX(z), n);
    }
    
    private double zTransformOfX(double z) {
        // Return the z-transform of X at z
    }
}
```
x??

